agda/counter/Completeness.agda
@@ -44,159 +44,6 @@ data _⇴_≗_ : List Type → Type → Type → Set where
 ≤d-to-≤a ≤d-top = ≤a-top
 ≤d-to-≤a (≤d-arr ≤d ≤d₁) = ≤a-arr (≤d-to-≤a ≤d) (≤d-to-≤a ≤d₁)
 
-----------------------------------------------------------------------
---+                                                                +--
---+                             Shift                              +--
---+                                                                +--
-----------------------------------------------------------------------
-
-↑Γ : (Γ : Context) → (n : ℕ) → (n ≤n length Γ) → Type → Context
-↑Γ Γ zero n≤l T = Γ , T
-↑Γ ∅ (suc n) () T
-↑Γ (Γ , A) (suc n) (s≤s n≤l) T = (↑Γ Γ n n≤l T) , A
-
-↓Γ : (Γ : Context) → (n : ℕ) → (n ≤n length Γ) → Context
-↓Γ ∅ .zero z≤n = ∅
-↓Γ (Γ , A) zero n≤l = Γ
-↓Γ (Γ , A) (suc n) (s≤s n≤l) = (↓Γ Γ n n≤l) , A
-
-↑Γ-var₁ : ∀ {Γ n A B x n≤l}
-  → Γ ∋ x ⦂ B
-  → n ≤n x
-  → ↑Γ Γ n n≤l A ∋ suc x ⦂ B
-↑Γ-var₁ {n = zero} x∈Γ n≤x = S x∈Γ
-↑Γ-var₁ {n = suc n} {n≤l = s≤s n≤l} (S x∈Γ) (s≤s n≤x) = S (↑Γ-var₁ x∈Γ n≤x)
-
-↑Γ-var₂ : ∀ {Γ n A B x n≤l}
-  → Γ ∋ x ⦂ B
-  → ¬ n ≤n x
-  → ↑Γ Γ n n≤l A ∋ x ⦂ B
-↑Γ-var₂ {n = zero} {x = zero} x∈Γ n>x = ⊥-elim (n>x z≤n)
-↑Γ-var₂ {n = zero} {x = suc x} x∈Γ n>x = ⊥-elim (n>x z≤n)
-↑Γ-var₂ {n = suc n} {x = zero} {s≤s n≤l} Z n>x = Z
-↑Γ-var₂ {Γ , C} {n = suc n} {x = suc x} {s≤s n≤l} (S x∈Γ) n>x = S (↑Γ-var₂ x∈Γ λ n≤x → n>x (s≤s n≤x))
-
-∋-weaken : ∀ {Γ A n x B}
-  → Γ ∋ x ⦂ B
-  → (n≤l : n ≤n length Γ)
-  → ↑Γ Γ n n≤l A ∋ ↑-var n x ⦂ B
-∋-weaken {Γ = Γ} {n = n} {x = x} x∈Γ n≤l with n ≤? x
-... | yes p = ↑Γ-var₁ x∈Γ p
-... | no ¬p = ↑Γ-var₂ x∈Γ ¬p
-
-⇧-⇧-comm : ∀ H m n → m ≤n n → H ⇧ m ⇧ suc n ≡ H ⇧ n ⇧ m
-⇧-⇧-comm (τ A) m n m≤n = refl
-⇧-⇧-comm (⟦ e ⟧⇒ H) m n m≤n rewrite ↑-↑-comm e m n m≤n | ⇧-⇧-comm H m n m≤n = refl
-
-postulate
-
-{-
-⊢a-strengthen : ∀ {Γ e A B n}
-  → Γ , A ⊢a H ⇛ e ⇛ B
-  → ¬ (e ≡ var n)
-  → Γ ⊢a H ⇩ n ⇛ e ↓ n ⇛ B
--}
-  ⊢a-strengthen : ∀ {Γ e H A B}
-    → Γ , A ⊢a H ⇧ 0 ⇛ e ↑ 0 ⇛ B
-    → Γ ⊢a H ⇛ e ⇛ B
-    
-  ≤a-strengthen : ∀ {Γ A B H}
-    → Γ , A ⊢a B ≤ (H ⇧ 0)
-    → Γ ⊢a B ≤ H
-
-  ≤a-weaken : ∀ {Γ A B H}
-    → Γ ⊢a B ≤ H
-    → Γ , A ⊢a B ≤ (H ⇧ 0)
-
-  ⊢a-weaken : ∀ {Γ e H A B}
-    → Γ ⊢a H ⇛ e ⇛ B
-    → Γ , A ⊢a H ⇧ 0 ⇛ e ↑ 0 ⇛ B
-
-≤a-strengthen-gen : ∀ {Γ A B H n n≤l}
-  → ↑Γ Γ n n≤l A ⊢a B ≤ (H ⇧ n)
-  → Γ ⊢a B ≤ H
-≤a-strengthen-gen B≤H = {!!}
-
-≤a-strengthen-gen' : ∀ {Γ A H n n≤l}
-  → Γ ⊢a A ≤ H
-  → ↓Γ Γ n n≤l ⊢a A ≤ (H ⇩ n)
-  
-⊢a-strengthen-gen' : ∀ {Γ A H n n≤l e}
-  → Γ ⊢a H ⇛ e ⇛ A
-  → ↓Γ Γ n n≤l ⊢a (H ⇩ n) ⇛ e ↓ n ⇛ A
-
-≤a-strengthen-gen' ≤a-int = ≤a-int
-≤a-strengthen-gen' ≤a-top = ≤a-top
-≤a-strengthen-gen' (≤a-arr A≤H A≤H₁) = ≤a-arr (≤a-strengthen-gen' A≤H) (≤a-strengthen-gen' A≤H₁)
-≤a-strengthen-gen' (≤a-hint ⊢e A≤H) = ≤a-hint (⊢a-strengthen-gen' ⊢e) (≤a-strengthen-gen' A≤H)
-
-⊢a-strengthen-gen' (⊢a-lit x) = ⊢a-lit (≤a-strengthen-gen' x)
-⊢a-strengthen-gen' (⊢a-var x∈Γ A≤H) = ⊢a-var {!!} (≤a-strengthen-gen' A≤H)
-⊢a-strengthen-gen' (⊢a-app ⊢e) = {!!}
-⊢a-strengthen-gen' (⊢a-ann ⊢e x) = {!!}
-⊢a-strengthen-gen' (⊢a-lam₁ ⊢e) = ⊢a-lam₁ (⊢a-strengthen-gen' ⊢e)
-⊢a-strengthen-gen' (⊢a-lam₂ ⊢e ⊢e₁) = ⊢a-lam₂ (⊢a-strengthen-gen' ⊢e) {!⊢a-strengthen-gen' ⊢e₁!}
-
-↓Γ-var₁ : ∀ {Γ n x A n≤l}
-  → Γ ∋ x ⦂ A
-  → suc n ≤n x
-  → ↓Γ Γ n n≤l ∋ pred x ⦂ A
-↓Γ-var₁ {Γ , B} {zero} (S x∈Γ) (s≤s n+1≤x) = {!!}
-↓Γ-var₁ {Γ , B} {suc n} {n≤l = s≤s n≤l} (S x∈Γ) (s≤s n+1≤x) = {!↓Γ-var₁ x∈Γ n+1≤x!}
-
-
-∋-strenghthen : ∀ {Γ n x A}
-  → Γ ∋ x ⦂ A
-  → (n≤l : n ≤n length Γ)
-  → ↓Γ Γ n n≤l ∋ ↓-var n x ⦂ A
-∋-strenghthen {Γ , B} {n} {x} {A} x∈Γ n≤l with suc n ≤? x
-... | yes p = {!!}
-... | no ¬p = {!!}
-
-≤a-weaken-gen : ∀ {Γ A B H n n≤l}
-  → Γ ⊢a B ≤ H
-  → ↑Γ Γ n n≤l A ⊢a B ≤ (H ⇧ n)
-  
-⊢a-weaken-gen : ∀ {Γ e H A B n n≤l}
-  → Γ ⊢a H ⇛ e ⇛ B
-  → ↑Γ Γ n n≤l A ⊢a H ⇧ n ⇛ e ↑ n ⇛ B
-
-≤a-weaken-gen ≤a-int = ≤a-int
-≤a-weaken-gen ≤a-top = ≤a-top
-≤a-weaken-gen (≤a-arr B≤H B≤H₁) = ≤a-arr (≤a-weaken-gen B≤H) (≤a-weaken-gen B≤H₁)
-≤a-weaken-gen (≤a-hint ⊢e B≤H) = ≤a-hint (⊢a-weaken-gen ⊢e) (≤a-weaken-gen B≤H)
-
-eq-sample : ∀ H n
-  → H ⇧ n ⇧ 0 ≡ H ⇧ 0 ⇧ (suc n)
-eq-sample H n rewrite ⇧-⇧-comm H 0 n z≤n = refl
-
-⊢a-weaken-gen (⊢a-lit B≤H) = ⊢a-lit (≤a-weaken-gen B≤H)
-⊢a-weaken-gen {n = n} {n≤l} (⊢a-var {x = x} x∈Γ B≤H) = ⊢a-var (∋-weaken x∈Γ n≤l) (≤a-weaken-gen B≤H)
-⊢a-weaken-gen (⊢a-app ⊢e) = ⊢a-app (⊢a-weaken-gen ⊢e)
-⊢a-weaken-gen (⊢a-ann ⊢e B≤H) = ⊢a-ann (⊢a-weaken-gen ⊢e) (≤a-weaken-gen B≤H)
-⊢a-weaken-gen {n≤l = n≤l} (⊢a-lam₁ ⊢e) = ⊢a-lam₁ (⊢a-weaken-gen {n≤l = s≤s n≤l} ⊢e)
-⊢a-weaken-gen {H = ⟦ _ ⟧⇒ H} {A = A} {n = n} {n≤l = n≤l} (⊢a-lam₂ ⊢e ⊢f) with ⊢a-weaken-gen {A = A} {n = suc n} {n≤l = s≤s n≤l} ⊢f
-... | ind-f rewrite sym (eq-sample H n) = ⊢a-lam₂ (⊢a-weaken-gen ⊢e) ind-f
-
-{-
-
--- we need to gen the weakening, possibly to alter context into a list
-
-≤a-weaken ≤a-int = ≤a-int
-≤a-weaken ≤a-top = ≤a-top
-≤a-weaken (≤a-arr {A = A} C≤A B≤D) = ≤a-arr (≤a-weaken C≤A) (≤a-weaken B≤D)
-≤a-weaken (≤a-hint {A = A} ⊢e B≤H) = ≤a-hint (⊢a-weaken ⊢e) (≤a-weaken B≤H)
-
-⊢a-weaken (⊢a-lit ≤a-int) = ⊢a-lit ≤a-int
-⊢a-weaken (⊢a-lit ≤a-top) = ⊢a-lit ≤a-top
-⊢a-weaken (⊢a-var {x = x} x∈Γ B≤H) = ⊢a-var (S x∈Γ) (≤a-weaken B≤H)
-⊢a-weaken (⊢a-app ⊢e) = ⊢a-app (⊢a-weaken ⊢e)
-⊢a-weaken (⊢a-ann ⊢e B≤H) = ⊢a-ann (⊢a-weaken ⊢e) (≤a-weaken B≤H)
-⊢a-weaken (⊢a-lam₁ ⊢e) = ⊢a-lam₁ {!⊢a-weaken ⊢e!}
-⊢a-weaken (⊢a-lam₂ ⊢e ⊢f) = ⊢a-lam₂ (⊢a-weaken ⊢e) {!⊢a-weaken ⊢f!}
-
--}
-
 spl-weaken : ∀ {H A es T As A' n}
   → ❪ H , A ❫↣❪ es , T , As , A' ❫
   → ❪ H ⇧ n , A ❫↣❪ map (_↑ n) es , T , As , A' ❫
@@ -239,7 +86,7 @@ subsumption : ∀ {Γ H e A H' H'' es As A'}
 ... | ≤a-hint x A≤H = A≤H
 ⊢a-to-≤a (⊢a-ann ⊢a x) = x
 ⊢a-to-≤a (⊢a-lam₁ ⊢a) = ≤a-arr ≤a-refl-τ (≤a-strengthen-τ (⊢a-to-≤a ⊢a))
-⊢a-to-≤a (⊢a-lam₂ ⊢a ⊢a₁) = ≤a-hint (rebase ⊢a ≤a-refl-τ) (≤a-strengthen (⊢a-to-≤a ⊢a₁))
+⊢a-to-≤a (⊢a-lam₂ ⊢a ⊢a₁) = ≤a-hint (rebase ⊢a ≤a-refl-τ) (≤a-strengthen-0 (⊢a-to-≤a ⊢a₁))
   where
     rebase : ∀ {Γ e A B}
       → Γ ⊢a τ Top ⇛ e ⇛ B
@@ -253,7 +100,7 @@ subsumption (⊢a-app ⊢e) spl ch sub with ⊢a-to-≤a ⊢e
 ... | ≤a-hint ⊢e₂ res = ⊢a-app (subsumption ⊢e (have spl) (ch-cons ch) (≤a-hint ⊢e₂ sub))
 
 subsumption (⊢a-ann ⊢e x) spl ch sub = ⊢a-ann ⊢e sub
-subsumption (⊢a-lam₂ ⊢e ⊢f) (have spl) (ch-cons ch) (≤a-hint x sub) = ⊢a-lam₂ ⊢e (subsumption ⊢f (spl-weaken spl) (ch-weaken ch) (≤a-weaken sub))
+subsumption (⊢a-lam₂ ⊢e ⊢f) (have spl) (ch-cons ch) (≤a-hint x sub) = ⊢a-lam₂ ⊢e (subsumption ⊢f (spl-weaken spl) (ch-weaken ch) (≤a-weaken {n≤l = z≤n} sub))
 
 rebase-≤ : ∀ {Γ A A' As H H' e es T₁ T₂}
   → Γ ⊢a A ≤ H
@@ -282,7 +129,7 @@ rebase-gen (⊢a-var x∈Γ A≤H) spl ⊢e ch = ⊢a-var x∈Γ (rebase-≤ A�
 rebase-gen (⊢a-app ⊢f) spl ⊢e ch = ⊢a-app (rebase-gen ⊢f (have spl) ⊢e (ch-cons ch))
 rebase-gen (⊢a-ann ⊢f A≤H) spl ⊢e ch = ⊢a-ann ⊢f (rebase-≤ A≤H spl ch ⊢e)
 rebase-gen (⊢a-lam₁ ⊢f) none ⊢e ch-none = ⊢a-lam₂ ⊢e ⊢f
-rebase-gen (⊢a-lam₂ ⊢f ⊢a) (have spl) ⊢e (ch-cons ch) = ⊢a-lam₂ ⊢f (rebase-gen ⊢a (spl-weaken spl) (⊢a-weaken ⊢e) (ch-weaken ch))
+rebase-gen (⊢a-lam₂ ⊢f ⊢a) (have spl) ⊢e (ch-cons ch) = ⊢a-lam₂ ⊢f (rebase-gen ⊢a (spl-weaken spl) (⊢a-weaken {n≤l = z≤n} ⊢e) (ch-weaken ch))
 
 rebase-gen-1 : ∀ {Γ e₁ e₂ A B C D}
   → Γ ⊢a τ (A ⇒ B) ⇛ e₁ ⇛ C ⇒ D
