agda/counter/Prelude.agda
@@ -6,7 +6,7 @@ open import Data.String using (String) public
 open import Relation.Nullary using (yes; no; Dec; ¬_) public
 open import Relation.Nullary.Decidable using (True; toWitness; fromWitness) public
 open import Function.Base using (case_of_; case_return_of_) public
-open import Relation.Binary.PropositionalEquality using (_≡_; refl; cong; sym) public
+open import Relation.Binary.PropositionalEquality using (_≡_; _≢_; refl; cong; sym; ≢-sym) public
 open import Data.Empty public
 open import Data.Product using (_×_; proj₁; proj₂; ∃; ∃-syntax) renaming (_,_ to ⟨_,_⟩) public
 open import Data.List using (List; []; _∷_; _++_; length; reverse; map; foldr; downFrom) public
@@ -33,3 +33,9 @@ m≰n⇒n<m {zero} {zero} m≰n = ⊥-elim (m≰n z≤n)
 m≰n⇒n<m {zero} {suc n} m≰n = ⊥-elim (m≰n z≤n)
 m≰n⇒n<m {suc m} {zero} m≰n = s≤s z≤n
 m≰n⇒n<m {suc m} {suc n} m≰n = s≤s (m≰n⇒n<m {m} {n} (m+1≰n+1⇒m≰n m≰n))
+
+n<m⇒m≰n : ∀ {m n}
+  → n < m
+  → m ≰ n
+n<m⇒m≰n {suc m} {zero} n<m = λ ()
+n<m⇒m≰n {suc m} {suc n} (s≤s n<m) (s≤s m≤n) = n<m⇒m≰n {m} {n} n<m m≤n
